wip

src/prop/PFConsistentStrong.v
@@ -27,6 +27,7 @@ Require Import PromiseConsistent.
 Require Import PFConsistent.
 Require Import ReorderCancel.
 Require Import MemoryProps.
+Require Import OrderedTimes.
 
 Set Implicit Arguments.
 
@@ -263,8 +264,331 @@ Proof.
   erewrite Memory.bot_get in *. clarify.
 Qed.
 
-Definition pf_consistent_flex lang (e0:Thread.t lang): Prop :=
-  exists tr times,
+
+
+
+Definition pf_consistent_flex lang (e0:Thread.t lang)
+           (tr : list (ThreadEvent.t * Memory.t)) (times : Loc.t -> list Time.t)
+           (f: Loc.t -> nat -> (Time.t -> Time.t -> Prop))
+  : Prop :=
+  (<<MAP: forall loc n
+                 (TS: Time.lt (Memory.max_ts loc e0.(Thread.memory)) (incr_time_seq n)),
+      cap_flex_map_loc
+        (Memory.max_ts loc e0.(Thread.memory))
+        (Time.incr (Memory.max_ts loc e0.(Thread.memory)))
+        (incr_time_seq n) (times loc) (f loc n)>>) /\
+  (<<CONSISTENT: forall mem1 (tm: Loc.t -> nat)
+                        (TM: forall loc, Time.lt (Memory.max_ts loc e0.(Thread.memory)) (incr_time_seq (tm loc)))
+                        (CAP: cap_flex e0.(Thread.memory) mem1 (fun loc => incr_time_seq (tm loc))),
+      exists ftr e1,
+        (<<STEPS: traced_step ftr (Thread.mk _ e0.(Thread.state) e0.(Thread.local) TimeMap.bot mem1) e1>>) /\
+        (<<EVENTS: List.Forall (fun em => <<SAT: (promise_free /1\ no_sc /1\ write_not_in (fun loc ts => (<<TS: Time.le ts (incr_time_seq (tm loc))>>) /\ (<<PROM: ~ covered loc ts e0.(Thread.local).(Local.promises)>>))) (fst em)>> /\ <<TAU: ThreadEvent.get_machine_event (fst em) = MachineEvent.silent>>) ftr >>) /\
+        (<<TRACE: List.Forall2 (fun em fem => <<EVENT: tevent_map (fun loc => f loc (tm loc)) (fst fem) (fst em)>> /\ <<MEM: memory_map (fun loc => f loc (tm loc)) (snd em) (snd fem)>>) tr ftr>>) /\
+        (__guard__((exists st',
+                       (<<LOCAL: Local.failure_step e1.(Thread.local)>>) /\
+                       (<<FAILURE: Language.step lang ProgramEvent.failure (@Thread.state lang e1) st'>>)) \/
+                   ((<<PROMISES: e1.(Thread.local).(Local.promises) = Memory.bot>>) /\
+                    (<<WRITES: forall loc from to val released
+                                      (GET: Memory.get loc to e0.(Thread.local).(Local.promises) = Some (from, Message.concrete val released)),
+                        exists e m,
+                          (<<WRITING: promise_writing_event loc from to val released e>>) /\
+                          (<<IN: List.In (e, m) ftr>>)>>))))>>).
+
+Lemma pf_consistent_strong_aux_pf_consistent_flex lang (th: Thread.t lang)
+      (WF: Local.wf th.(Thread.local) th.(Thread.memory))
+      (MEM: Memory.closed th.(Thread.memory))
+      (CONSISTENT: pf_consistent_strong_aux th)
+  :
+    exists tr times f, <<CONSISTENT: pf_consistent_flex th tr times f>>.
+Proof.
+  exploit Memory.cap_exists; eauto. i. des.
+  exploit CONSISTENT; eauto. i. des. exists tr, times.
+  hexploit (@choice
+              (Loc.t * nat)
+              (Time.t -> Time.t -> Prop)
+              (fun locn f =>
+                 let (loc, n) := locn in
+                 forall
+                   (TS: Time.lt (Memory.max_ts loc th.(Thread.memory)) (incr_time_seq n)),
+                   cap_flex_map_loc
+                     (Memory.max_ts loc th.(Thread.memory))
+                     (Time.incr (Memory.max_ts loc th.(Thread.memory)))
+                     (incr_time_seq n) (times loc) f)).
+  { intros [loc n].
+    destruct (classic (Time.lt (Memory.max_ts loc th.(Thread.memory)) (incr_time_seq n))).
+    { des. hexploit cap_flex_map_loc_exists.
+      { eapply Time.incr_spec. }
+      { eapply H. }
+      i. des. eauto. }
+    { exists bot2. i. exfalso. eapply H. auto. }
+  }
+  intros [f SPEC]. des. exists (fun loc ts => f (loc, ts)). econs.
+  { ii. specialize (SPEC (loc, n)). ss. eauto. }
+  ii. assert (MAP: cap_flex_map
+                     (Memory.max_timemap (Thread.memory th))
+                     (fun loc => Time.incr (Memory.max_ts loc (Thread.memory th)))
+                     (fun loc => incr_time_seq (tm loc))
+                     times (fun loc => f (loc, tm loc))).
+  { eapply cap_flex_map_locwise. i.
+    eapply (SPEC (loc, tm loc)). eauto. }
+  destruct e1. ss.
+  hexploit traced_steps_map.
+  { eapply mapping_map_lt_map_le. eapply MAP. }
+  { eapply MAP. }
+  { eapply mapping_map_lt_map_eq. eapply MAP. }
+  { eapply wf_time_mapped_mappable.
+    { eapply List.Forall_impl; eauto. i. ss. des; eauto. }
+    { eapply cap_flex_map_complete; eauto. }
+  }
+  { eapply STEPS. }
+  { ss. }
+  { ss. }
+  { ss. }
+  { eapply Local.cap_wf; eauto. }
+  { instantiate (1:=mem1). instantiate (1:=th.(Thread.local)).
+    eapply cap_flex_wf; eauto. }
+  { eapply cap_flex_closed; eauto. }
+  { eapply Memory.cap_closed; eauto. }
+  { eapply Memory.closed_timemap_bot.
+    eapply cap_flex_closed in CAP0; auto. eapply CAP0. }
+  { eapply Memory.closed_timemap_bot.
+    eapply Memory.cap_closed in CAP; auto. eapply CAP. }
+  { eapply map_ident_in_memory_local.
+    { ii. eapply MAP. eapply TS. }
+    { eapply MAP. }
+    { eauto. }
+    { eauto. }
+  }
+  { eapply concrete_messages_le_cap_flex_memory_map.
+    { refl. }
+    { instantiate (1:=(fun loc => Time.incr (Memory.max_ts loc th.(Thread.memory)))).
+      i. eapply Time.incr_spec. }
+    { eapply TM. }
+    { eapply cap_cap_flex; eauto. }
+    { eauto. }
+    { eauto. }
+    { eauto. }
+    { eauto. }
+  }
+  { eapply mapping_map_lt_collapsable_unwritable. eapply MAP. }
+  { eapply timemap_bot_map. eapply MAP. }
+  { refl. } i. des.
+  exploit write_not_in_traced; eauto.
+  { ss. transitivity (th.(Thread.memory)).
+    { eapply WF. }
+    { eapply CAP0. }
+  } intros NOTIN. ss.
+  exists ftr, (Thread.mk _ state flc1 fsc1 fmem1). splits; auto.
+  { eapply List.Forall_forall. i.
+    cut ((promise_free /1\ no_sc) (fst x) /\ ThreadEvent.get_machine_event (fst x) = MachineEvent.silent).
+    { i. des. splits; auto. eapply List.Forall_forall in H; eauto. ss.
+      eapply write_not_in_mon_bot; eauto. intros loc ts. intros. des.
+      assert (ITV: Interval.mem (Time.bot, incr_time_seq (tm loc)) ts).
+      { econs; ss. }
+      erewrite (@cap_flex_covered _ _ (fun loc => incr_time_seq (tm loc))) in ITV; eauto.
+      inv ITV. econs; eauto. econs; eauto.
+      destruct (Memory.get loc to (Local.promises (Thread.local th)))
+        as [[from' msg']|] eqn:GETPROM; eauto.
+      exfalso. dup GETPROM.
+      eapply WF in GETPROM. eapply CAP0 in GETPROM. clarify.
+      eapply SAT0. econs; eauto.
+    }
+    eapply list_Forall2_in in H; eauto. des.
+    eapply List.Forall_forall in IN; eauto. ss. des.
+    destruct x, a. ss. inv EVENT; ss. inv KIND; ss.
+    splits; auto. inv MSG0; ss. inv MSG; ss. inv MAP1; ss.
+  }
+  { ss. unguard. des; eauto.
+    { left. esplits; eauto. eapply failure_step_map; eauto.
+      { eapply mapping_map_lt_map_le. eapply MAP. }
+      { eapply mapping_map_lt_map_eq. eapply MAP. }
+    }
+    { right. splits.
+      { inv LOCAL. erewrite PROMISES in *. eapply bot_promises_map; eauto. }
+      { i. exploit WRITES; eauto. i. des.
+        eapply list_Forall2_in2 in IN; eauto. des.
+        destruct b. ss. eexists t, _. splits; eauto.
+        eapply promise_writing_event_map; eauto.
+        { inv WF. eapply PROMISES0 in GET. eauto. }
+        { eapply MAP. }
+        { ii. eapply MAP. auto. }
+      }
+    }
+  }
+Qed.
+
+Definition pf_consistent_flex_aux lang (e0:Thread.t lang)
+           (tr : list (ThreadEvent.t * Memory.t)) (times : Loc.t -> list Time.t)
+           (f: Loc.t -> nat -> (Time.t -> Time.t -> Prop))
+  : Prop :=
+  (<<MAP: forall loc n
+                 (TS: Time.lt (Memory.max_ts loc e0.(Thread.memory)) (incr_time_seq n)),
+      cap_flex_map_loc
+        (Memory.max_ts loc e0.(Thread.memory))
+        (Time.incr (Memory.max_ts loc e0.(Thread.memory)))
+        (incr_time_seq n) (times loc) (f loc n)>>) /\
+  (<<CONSISTENT: forall mem1
+                        (tm: Loc.t -> nat)
+                        (FUTURE: Memory.future_weak e0.(Thread.memory) mem1)
+                        (CLOSED: Memory.closed mem1)
+                        (LOCAL: Local.wf e0.(Thread.local) mem1)
+                        (TM0: forall loc, Time.lt (Memory.max_ts loc e0.(Thread.memory)) (incr_time_seq (tm loc)))
+                        (TM1: forall loc, Time.lt (Memory.max_ts loc mem1) (incr_time_seq (tm loc))),
+      exists ftr e1,
+        (<<STEPS: traced_step ftr (Thread.mk _ e0.(Thread.state) e0.(Thread.local) TimeMap.bot mem1) e1>>) /\
+        (<<EVENTS: List.Forall (fun em => <<SAT: (promise_free /1\ no_sc /1\ write_not_in (fun loc ts => (<<TS: Time.le ts (incr_time_seq (tm loc))>>) /\ (<<PROM: ~ covered loc ts e0.(Thread.local).(Local.promises)>>))) (fst em)>> /\ <<TAU: ThreadEvent.get_machine_event (fst em) = MachineEvent.silent>>) ftr >>) /\
+        (<<TRACE: List.Forall2 (fun em fem => tevent_map (fun loc => f loc (tm loc)) (fst fem) (fst em)) tr ftr>>) /\
+        (__guard__((exists st',
+                       (<<LOCAL: Local.failure_step e1.(Thread.local)>>) /\
+                       (<<FAILURE: Language.step lang ProgramEvent.failure (@Thread.state lang e1) st'>>)) \/
+                   ((<<PROMISES: e1.(Thread.local).(Local.promises) = Memory.bot>>) /\
+                    (<<WRITES: forall loc from to val released
+                                      (GET: Memory.get loc to e0.(Thread.local).(Local.promises) = Some (from, Message.concrete val released)),
+                        exists e m,
+                          (<<WRITING: promise_writing_event loc from to val released e>>) /\
+                          (<<IN: List.In (e, m) ftr>>)>>))))>>).
+
+Lemma pf_consistent_flex_pf_consistent_flex_aux lang (th: Thread.t lang) tr times f
+      (WF: Local.wf th.(Thread.local) th.(Thread.memory))
+      (MEM: Memory.closed th.(Thread.memory))
+      (CONSISTENT: pf_consistent_flex th tr times f)
+  :
+    pf_consistent_flex_aux th tr times f.
+Proof.
+  unfold pf_consistent_flex in *. des. econs; eauto.
+  ii. exploit (@cap_flex_exists th.(Thread.memory) (fun loc => incr_time_seq (tm loc))); eauto. i. des.
+  exploit CONSISTENT0; eauto. i. des. destruct e1. ss.
+  hexploit traced_steps_map.
+  { eapply ident_map_le; eauto. }
+  { eapply ident_map_bot; eauto. }
+  { eapply ident_map_eq; eauto. }
+  { eapply List.Forall_forall. i. eapply ident_map_mappable_evt. }
+  { eapply STEPS. }
+  { ss. }
+  { ss. }
+  { ss. }
+  { eapply cap_flex_wf; eauto. }
+  { eapply LOCAL. }
+  { eauto. }
+  { eapply cap_flex_closed; eauto. }
+  { eapply Memory.closed_timemap_bot. inv CLOSED. auto. }
+  { eapply Memory.closed_timemap_bot.
+    eapply cap_flex_closed in CAP; eauto. eapply CAP. }
+  { eapply ident_map_local. }
+  { eapply cap_flex_future_memory_map; try apply CAP; eauto.
+    ii. left. eauto. }
+  { eapply mapping_map_lt_collapsable_unwritable. eapply ident_map_lt. }
+  { eapply timemap_bot_map. eapply ident_map_bot. }
+  { refl. }
+  i. des. exists ftr0, (Thread.mk _ state flc1 fsc1 fmem1).
+  splits; auto.
+  { eapply List.Forall_forall. i.
+    cut ((promise_free /1\ no_sc) (fst x) /\ ThreadEvent.get_machine_event (fst x) = MachineEvent.silent).
+    { i. des. splits; auto.
+      eapply list_Forall2_in in H; eauto. des.
+      eapply List.Forall_forall in IN; eauto. ss. des.
+      eapply ident_map_write_not_in; eauto. }
+    eapply list_Forall2_in in H; eauto. des.
+    eapply List.Forall_forall in IN; eauto. ss. des.
+    destruct x, a. ss. inv EVENT; ss. inv KIND; ss.
+    splits; auto. inv MSG0; ss. inv MSG; ss. inv MAP1; ss. }
+    { eapply list_Forall2_compose; eauto.
+    i. ss. des. eapply ident_map_compose_tevent; eauto. }
+  { ss. unguard. des; eauto.
+    { left. esplits; eauto. eapply failure_step_map; eauto.
+      { eapply ident_map_le. }
+      { eapply ident_map_eq. }
+    }
+    { right. splits.
+      { inv LOCAL0. erewrite PROMISES in *. eapply bot_promises_map; eauto. }
+      { i. exploit WRITES; eauto. i. des.
+        eapply list_Forall2_in2 in IN; eauto. des.
+        destruct b. ss. eexists t, _. splits; eauto.
+        eapply promise_writing_event_map; eauto.
+        { inv LOCAL. eapply PROMISES0 in GET. eauto. }
+        { eapply ident_map_lt. }
+        { ii. ss. }
+      }
+    }
+  }
+Qed.
+
+Definition pf_consistent_super_strong lang (e0:Thread.t lang)
+           (tr : list (ThreadEvent.t * Memory.t)) (times : Loc.t -> list Time.t): Prop :=
+  forall mem1 tm sc
+         (FUTURE: Memory.future_weak e0.(Thread.memory) mem1)
+         (CLOSED: Memory.closed mem1)
+         (LOCAL: Local.wf e0.(Thread.local) mem1)
+         (TM0: forall loc, Time.lt (Memory.max_ts loc e0.(Thread.memory)) (tm loc))
+         (TM1: forall loc, Time.lt (Memory.max_ts loc mem1) (tm loc)),
+  exists ftr e1 f,
+    (<<STEPS: traced_step ftr (Thread.mk _ e0.(Thread.state) e0.(Thread.local) sc mem1) e1>>) /\
+    (<<EVENTS: List.Forall (fun em => <<SAT: (promise_free /1\ no_sc) (fst em)>> /\ <<TAU: ThreadEvent.get_machine_event (fst em) = MachineEvent.silent>>) ftr >>) /\
+    (<<MAP: cap_flex_map
+              (Memory.max_timemap e0.(Thread.memory))
+              (fun loc => Time.incr (Memory.max_ts loc e0.(Thread.memory)))
+              tm times f>>) /\
+    (<<TRACE: List.Forall2 (fun em fem => tevent_map f (fst fem) (fst em)) tr ftr>>) /\
+    (<<GOOD: good_future tm mem1 e1.(Thread.memory)>>) /\
+    (<<SC: e1.(Thread.sc) = sc>>) /\
+    (__guard__((exists st',
+                   (<<LOCAL: Local.failure_step e1.(Thread.local)>>) /\
+                   (<<FAILURE: Language.step lang ProgramEvent.failure (@Thread.state lang e1) st'>>)) \/
+               ((<<PROMISES: e1.(Thread.local).(Local.promises) = Memory.bot>>) /\
+                (<<WRITES: forall loc from to val released
+                                  (GET: Memory.get loc to e0.(Thread.local).(Local.promises) = Some (from, Message.concrete val released)),
+                    exists e m,
+                      (<<WRITING: promise_writing_event loc from to val released e>>) /\
+                      (<<IN: List.In (e, m) ftr>>)>>)))).
+
+
+wf_time_evt
+
+mappable_evt
+
+Lemma pf_consistent_flex_aux_pf_consistent_super_strong lang (th: Thread.t lang) tr times
+      (WF: Local.wf th.(Thread.local) th.(Thread.memory))
+      (MEM: Memory.closed th.(Thread.memory))
+      (CONSISTENT: pf_consistent_flex_aux th tr times)
+  :
+    pf_consistent_super_strong th tr times.
+Proof.
+  ii. exploit CONSISTENT; eauto. i. des. destruct e1.
+  exploit write_not_in_good_future_traced; try apply STEPS; ss; auto.
+  { eapply Memory.closed_timemap_bot. inv CLOSED. auto. }
+  { eapply List.Forall_impl; eauto. i. ss. des. eapply write_not_in_mon; eauto.
+    i. ss. des. split; auto. ii. eapply PROM.
+    inv H. econs; eauto. eapply LOCAL in GET; eauto. }
+  eapply no_sc_any_sc_traced in STEPS; ss; cycle 1.
+  { i. eapply List.Forall_forall in IN; eauto. ss. des; auto. } des.
+  esplits; eauto.
+  { eapply List.Forall_impl; [|apply EVENTS]. i. ss. des; auto. }
+  { eapply no_sc_same_sc_traced in STEPS0; eauto.
+    eapply List.Forall_impl; eauto. i. ss. des; auto. }
+Qed.
+
+Lemma consistent_pf_consistent_super_strong lang (th: Thread.t lang)
+      (LOCAL: Local.wf th.(Thread.local) th.(Thread.memory))
+      (MEM: Memory.closed th.(Thread.memory))
+      (CONSISTENT: Thread.consistent th)
+  :
+    exists tr times, <<CONSISTENT: pf_consistent_super_strong th tr times>>.
+Proof.
+  eapply consistent_pf_consistent in CONSISTENT; eauto.
+  eapply pf_consistent_pf_consistent_strong in CONSISTENT; eauto.
+  eapply pf_consistent_strong_pf_consistent_strong_aux in CONSISTENT; eauto.
+  eapply pf_consistent_strong_aux_pf_consistent_flex in CONSISTENT; eauto. des.
+  eapply pf_consistent_flex_pf_consistent_flex_aux in CONSISTENT0; eauto.
+  eapply pf_consistent_flex_aux_pf_consistent_super_strong in CONSISTENT0; eauto.
+Qed.
+
+
+
+
+
+
+Definition pf_consistent_flex lang (e0:Thread.t lang)
+           (tr : list (ThreadEvent.t * Memory.t)) (times : Loc.t -> list Time.t): Prop :=
   forall mem1 tm
          (TM: forall loc, Time.lt (Memory.max_ts loc e0.(Thread.memory)) (tm loc))
          (CAP: cap_flex e0.(Thread.memory) mem1 tm),
@@ -291,7 +615,7 @@ Lemma pf_consistent_strong_aux_pf_consistent_flex lang (th: Thread.t lang)
       (MEM: Memory.closed th.(Thread.memory))
       (CONSISTENT: pf_consistent_strong_aux th)
   :
-    pf_consistent_flex th.
+    exists tr times, <<CONSISTENT: pf_consistent_flex th tr times>>.
 Proof.
   exploit Memory.cap_exists; eauto. i. des.
   exploit CONSISTENT; eauto. i. des.
@@ -388,8 +712,8 @@ Proof.
   }
 Qed.
 
-Definition pf_consistent_flex_aux lang (e0:Thread.t lang): Prop :=
-  exists (tr: list (ThreadEvent.t * Memory.t)) times,
+Definition pf_consistent_flex_aux lang (e0:Thread.t lang)
+           (tr : list (ThreadEvent.t * Memory.t)) (times : Loc.t -> list Time.t): Prop :=
   forall mem1 tm
          (FUTURE: Memory.future_weak e0.(Thread.memory) mem1)
          (CLOSED: Memory.closed mem1)
@@ -414,14 +738,13 @@ Definition pf_consistent_flex_aux lang (e0:Thread.t lang): Prop :=
                       (<<WRITING: promise_writing_event loc from to val released e>>) /\
                       (<<IN: List.In (e, m) ftr>>)>>)))).
 
-Lemma pf_consistent_flex_pf_consistent_flex_aux lang (th: Thread.t lang)
+Lemma pf_consistent_flex_pf_consistent_flex_aux lang (th: Thread.t lang) tr times
       (WF: Local.wf th.(Thread.local) th.(Thread.memory))
       (MEM: Memory.closed th.(Thread.memory))
-      (CONSISTENT: pf_consistent_flex th)
+      (CONSISTENT: pf_consistent_flex th tr times)
   :
-    pf_consistent_flex_aux th.
+    pf_consistent_flex_aux th tr times.
 Proof.
-  unfold pf_consistent_flex in *. des. exists tr, times.
   ii. exploit (@cap_flex_exists th.(Thread.memory) tm); eauto. i. des.
   exploit CONSISTENT; eauto. i. des. destruct e1. ss.
   hexploit traced_steps_map.
@@ -479,8 +802,8 @@ Proof.
   }
 Qed.
 
-Definition pf_consistent_super_strong lang (e0:Thread.t lang): Prop :=
-  exists (tr: list (ThreadEvent.t * Memory.t)) times,
+Definition pf_consistent_super_strong lang (e0:Thread.t lang)
+           (tr : list (ThreadEvent.t * Memory.t)) (times : Loc.t -> list Time.t): Prop :=
   forall mem1 tm sc
          (FUTURE: Memory.future_weak e0.(Thread.memory) mem1)
          (CLOSED: Memory.closed mem1)
@@ -507,14 +830,13 @@ Definition pf_consistent_super_strong lang (e0:Thread.t lang): Prop :=
                       (<<WRITING: promise_writing_event loc from to val released e>>) /\
                       (<<IN: List.In (e, m) ftr>>)>>)))).
 
-Lemma pf_consistent_flex_aux_pf_consistent_super_strong lang (th: Thread.t lang)
+Lemma pf_consistent_flex_aux_pf_consistent_super_strong lang (th: Thread.t lang) tr times
       (WF: Local.wf th.(Thread.local) th.(Thread.memory))
       (MEM: Memory.closed th.(Thread.memory))
-      (CONSISTENT: pf_consistent_flex_aux th)
+      (CONSISTENT: pf_consistent_flex_aux th tr times)
   :
-    pf_consistent_super_strong th.
+    pf_consistent_super_strong th tr times.
 Proof.
-  unfold pf_consistent_flex_aux in *. des. exists tr, times.
   ii. exploit CONSISTENT; eauto. i. des. destruct e1.
   exploit write_not_in_good_future_traced; try apply STEPS; ss; auto.
   { eapply Memory.closed_timemap_bot. inv CLOSED. auto. }
@@ -534,12 +856,12 @@ Lemma consistent_pf_consistent_super_strong lang (th: Thread.t lang)
       (MEM: Memory.closed th.(Thread.memory))
       (CONSISTENT: Thread.consistent th)
   :
-    pf_consistent_super_strong th.
+    exists tr times, <<CONSISTENT: pf_consistent_super_strong th tr times>>.
 Proof.
-  eapply pf_consistent_flex_aux_pf_consistent_super_strong; eauto.
-  eapply pf_consistent_flex_pf_consistent_flex_aux; eauto.
-  eapply pf_consistent_strong_aux_pf_consistent_flex; eauto.
-  eapply pf_consistent_strong_pf_consistent_strong_aux; eauto.
-  eapply pf_consistent_pf_consistent_strong; eauto.
-  eapply consistent_pf_consistent; eauto.
+  eapply consistent_pf_consistent in CONSISTENT; eauto.
+  eapply pf_consistent_pf_consistent_strong in CONSISTENT; eauto.
+  eapply pf_consistent_strong_pf_consistent_strong_aux in CONSISTENT; eauto.
+  eapply pf_consistent_strong_aux_pf_consistent_flex in CONSISTENT; eauto. des.
+  eapply pf_consistent_flex_pf_consistent_flex_aux in CONSISTENT0; eauto.
+  eapply pf_consistent_flex_aux_pf_consistent_super_strong in CONSISTENT0; eauto.
 Qed.
